code/k256/Hacl.K256.ECDSA.fsti
@@ -20,7 +20,8 @@ inline_for_extraction noextract
 let lbytes len = lbuffer uint8 len
 
 
-val ecdsa_sign_hashed_msg (signature:lbytes 64ul) (msgHash private_key nonce:lbytes 32ul) : Stack bool
+val ecdsa_sign_hashed_msg (signature:lbytes 64ul)
+  (msgHash private_key nonce:lbytes 32ul) : Stack bool
   (requires fun h ->
     live h msgHash /\ live h private_key /\ live h nonce /\ live h signature /\
     disjoint signature msgHash /\ disjoint signature private_key /\ disjoint signature nonce)
@@ -36,7 +37,8 @@ val ecdsa_verify_hashed_msg (msgHash:lbytes 32ul) (public_key signature:lbytes 6
     b == S.ecdsa_verify_hashed_msg (as_seq h0 msgHash) (as_seq h0 public_key) (as_seq h0 signature))
 
 
-val ecdsa_sign_sha256 (signature:lbytes 64ul) (msg_len:size_t) (msg:lbytes msg_len) (private_key nonce:lbytes 32ul) : Stack bool
+val ecdsa_sign_sha256 (signature:lbytes 64ul)
+  (msg_len:size_t) (msg:lbytes msg_len) (private_key nonce:lbytes 32ul) : Stack bool
   (requires fun h ->
     live h msg /\ live h private_key /\ live h nonce /\ live h signature /\
     disjoint signature msg /\ disjoint signature private_key /\ disjoint signature nonce)
@@ -78,3 +80,51 @@ val public_key_compressed_from_raw: pk:lbytes 33ul -> pk_raw:lbytes 64ul -> Stac
   (requires fun h -> live h pk /\ live h pk_raw /\ disjoint pk pk_raw)
   (ensures  fun h0 _ h1 -> modifies (loc pk) h0 h1 /\
     as_seq h1 pk == S.pk_compressed_from_raw (as_seq h0 pk_raw))
+
+
+///  Low-S normalization used in secp256k1
+
+val secp256k1_ecdsa_signature_normalize: signature: lbytes 64ul -> Stack bool
+  (requires fun h -> live h signature)
+  (ensures  fun h0 b h1 -> modifies (loc signature) h0 h1 /\
+    (let sgnt = S.secp256k1_ecdsa_signature_normalize (as_seq h0 signature) in
+    (b <==> Some? sgnt) /\ (b ==> (as_seq h1 signature == Some?.v sgnt))))
+
+val secp256k1_ecdsa_is_signature_normalized: signature: lbytes 64ul -> Stack bool
+  (requires fun h -> live h signature)
+  (ensures  fun h0 b h1 -> modifies0 h0 h1 /\
+    b == S.secp256k1_ecdsa_is_signature_normalized (as_seq h0 signature))
+
+
+val secp256k1_ecdsa_sign_hashed_msg (signature:lbytes 64ul)
+  (msgHash private_key nonce:lbytes 32ul) : Stack bool
+  (requires fun h ->
+    live h msgHash /\ live h private_key /\ live h nonce /\ live h signature /\
+    disjoint signature msgHash /\ disjoint signature private_key /\ disjoint signature nonce)
+  (ensures fun h0 b h1 -> modifies (loc signature) h0 h1 /\
+    (let sgnt = S.secp256k1_ecdsa_sign_hashed_msg (as_seq h0 msgHash) (as_seq h0 private_key) (as_seq h0 nonce) in
+    (b <==> Some? sgnt) /\ (b ==> (as_seq h1 signature == Some?.v sgnt))))
+
+
+val secp256k1_ecdsa_sign_sha256 (signature:lbytes 64ul)
+  (msg_len:size_t) (msg:lbytes msg_len) (private_key nonce:lbytes 32ul) : Stack bool
+  (requires fun h ->
+    live h msg /\ live h private_key /\ live h nonce /\ live h signature /\
+    disjoint signature msg /\ disjoint signature private_key /\ disjoint signature nonce)
+  (ensures fun h0 b h1 -> modifies (loc signature) h0 h1 /\
+    (let sgnt = S.secp256k1_ecdsa_sign_sha256 (v msg_len) (as_seq h0 msg) (as_seq h0 private_key) (as_seq h0 nonce) in
+    (b <==> Some? sgnt) /\ (b ==> (as_seq h1 signature == Some?.v sgnt))))
+
+
+val secp256k1_ecdsa_verify_hashed_msg (msgHash:lbytes 32ul) (public_key signature:lbytes 64ul) : Stack bool
+  (requires fun h ->
+    live h msgHash /\ live h public_key /\ live h signature)
+  (ensures fun h0 b h1 -> modifies0 h0 h1 /\
+    b == S.secp256k1_ecdsa_verify_hashed_msg (as_seq h0 msgHash) (as_seq h0 public_key) (as_seq h0 signature))
+
+
+val secp256k1_ecdsa_verify_sha256 (msg_len:size_t) (msg:lbytes msg_len) (public_key signature:lbytes 64ul) : Stack bool
+  (requires fun h ->
+    live h msg /\ live h public_key /\ live h signature)
+  (ensures fun h0 b h1 -> modifies0 h0 h1 /\
+    b == S.secp256k1_ecdsa_verify_sha256 (v msg_len) (as_seq h0 msg) (as_seq h0 public_key) (as_seq h0 signature))
